cava/Cava/Monad/SequentialProperties.v
@@ -1,0 +1,257 @@
+(****************************************************************************)
+(* Copyright 2020 The Project Oak Authors                                   *)
+(*                                                                          *)
+(* Licensed under the Apache License, Version 2.0 (the "License")           *)
+(* you may not use this file except in compliance with the License.         *)
+(* You may obtain a copy of the License at                                  *)
+(*                                                                          *)
+(*     http://www.apache.org/licenses/LICENSE-2.0                           *)
+(*                                                                          *)
+(* Unless required by applicable law or agreed to in writing, software      *)
+(* distributed under the License is distributed on an "AS IS" BASIS,        *)
+(* WITHOUT WARRANTIES OR CONDITIONS OF ANY KIND, either express or implied. *)
+(* See the License for the specific language governing permissions and      *)
+(* limitations under the License.                                           *)
+(****************************************************************************)
+
+Require Import Coq.Lists.List.
+Import ListNotations.
+Require Import ExtLib.Structures.Monads.
+Require Import ExtLib.Data.Monads.IdentityMonad.
+Export MonadNotation.
+
+Require Import Cava.Cava.
+Require Import Cava.Signal.
+Require Import Cava.Tactics.
+Require Import Cava.Acorn.Identity.
+Require Import Cava.Monad.CavaClass.
+Require Import Cava.Monad.Sequential.
+
+Require Import Coq.Arith.PeanoNat.
+Require Import Coq.micromega.Lia.
+Require Import Cava.ListUtils.
+
+(* Helpful tactics for simplifying sequential goals *)
+Ltac seqsimpl_step :=
+  first [ progress cbn beta iota delta
+                   [fst snd hd tl sequential SequentialSemantics]
+        | progress autorewrite with seqsimpl
+        | progress destruct_pair_let
+        | progress simpl_ident ].
+Ltac seqsimpl := repeat seqsimpl_step.
+
+Section Overlap.
+  Lemma overlap_cons1 {A} n (xs ys : seqType A) x :
+    n <= length xs ->
+    overlap n (x :: xs) ys = x :: overlap n xs (tl ys).
+  Proof.
+    intros; cbv [overlap]. cbn [length].
+    rewrite Nat.sub_succ_l by lia. rewrite app_comm_cons.
+    replace (n - length xs) with 0 by lia.
+    replace (n - S (length xs)) with 0 by lia.
+    cbn [repeat].
+    destruct ys; cbn [skipn tl];
+      [ rewrite skipn_nil; reflexivity | ].
+    reflexivity.
+  Qed.
+
+  Lemma overlap_cons2 {A} n (xs ys : seqType A) :
+    length xs <= n ->
+    overlap n xs ys = xs ++ repeat (defaultCombValue A) (n - length xs) ++ ys.
+  Proof.
+    intros; cbv [overlap]. cbn [length].
+    replace (length xs - n) with 0 by lia.
+    reflexivity.
+  Qed.
+
+  Lemma overlap_0_nil {A} (x : seqType A) : overlap 0 [] x = x.
+  Proof.
+    cbv [overlap]. cbn [length].
+    rewrite Nat.sub_0_l. cbn [skipn].
+    reflexivity.
+  Qed.
+
+  Lemma overlap_app_same {A} (x y : seqType A) :
+    overlap 0 x (x ++ y) = x ++ y.
+  Proof.
+    cbv [overlap]. rewrite Nat.sub_0_l, Nat.sub_0_r.
+    cbn [repeat]. rewrite skipn_app, Nat.sub_diag.
+    rewrite skipn_all.
+    cbn [skipn]. reflexivity.
+  Qed.
+
+  Lemma overlap_nil_r {A} n (x : seqType A) :
+    n <= length x -> overlap n x [] = x.
+  Proof.
+    intros. cbv [overlap]. cbn [length].
+    rewrite skipn_nil, app_nil_r.
+    replace (n - length x) with 0 by lia.
+    cbn [repeat]. rewrite app_nil_r.
+    reflexivity.
+  Qed.
+
+  Lemma overlap_assoc {A} n m (x y z : seqType A) :
+    overlap n x (overlap m y z) = overlap (n + m) (overlap n x y) z.
+  Proof.
+    cbv [overlap]. intros.
+    rewrite !app_assoc.
+    autorewrite with push_skipn push_length natsimpl.
+    rewrite <-!app_assoc.
+    change CombinationalMonad.combType with Signal.combType in *.
+    repeat (f_equal; try lia).
+  Qed.
+End Overlap.
+Hint Rewrite @overlap_cons1 @overlap_cons2 @overlap_nil_r
+     using solve [length_hammer] : seqsimpl.
+Hint Rewrite @overlap_0_nil @overlap_app_same using solve [eauto] : seqsimpl.
+
+Section Loops.
+  Lemma loopSeq'_step {A B C}
+        (f : seqType A * seqType C -> ident (seqType B * seqType C))
+        (spec : combType A -> combType C -> seqType B * seqType C) :
+    (forall a c, sequential (f ([a], [c])) = spec a c) ->
+    forall (loop_state : nat * ident (seqType B * seqType C)) a,
+      loopSeq' f loop_state a
+      = let t := fst loop_state in
+        let '(acc, feedback) := unIdent (snd loop_state) in
+        let c := hd (defaultCombValue C) feedback in
+        let r := spec a c in
+        (S t, ret (overlap t acc (fst r), overlap 0 (tl feedback) (snd r))).
+  Proof.
+    cbv [sequential loopSeq' SequentialSemantics]. intro Hfspec.
+    intros. seqsimpl. rewrite Hfspec. reflexivity.
+  Qed.
+
+  Lemma loop_stepwise {A B C}
+        (f : seqType A * seqType C -> ident (seqType B * seqType C))
+        (spec : combType A -> combType C -> seqType B * seqType C)
+        input :
+    (forall a c, sequential (f ([a], [c])) = spec a c) ->
+    sequential (loop (CavaSeq:=SequentialSemantics) f input)
+    = snd (fst (fold_left (fun loop_state a =>
+                             let '(t, acc, feedback) := loop_state in
+                             let c := hd (defaultCombValue C) feedback in
+                             let r := spec a c in
+                             (S t, overlap t acc (fst r), overlap 0 (tl feedback) (snd r)))
+                          input (0, [], [defaultCombValue C]))).
+  Proof.
+    cbv [loop loopSeq SequentialSemantics sequential]; intros.
+    seqsimpl.
+    erewrite fold_left_ext with (f0:=loopSeq' _) by (apply loopSeq'_step; eassumption).
+    factor_out_loops.
+    eapply fold_left_double_invariant
+      with(I:=fun (x : nat * seqType B * seqType C) (y : nat * ident (seqType B * seqType C)) =>
+                x = (fst y, fst (unIdent (snd y)), snd (unIdent (snd y)))).
+    { (* invariant holds at start *)
+      reflexivity. }
+    { (* invariant holds through loop *)
+    intros; repeat destruct_pair_let. subst.
+    seqsimpl. reflexivity. }
+  { (* invariant implies postcondition *)
+    intros. subst. seqsimpl. reflexivity. }
+  Qed.
+
+  Lemma loop_stepwise_indexed {A B C}
+        (f : seqType A * seqType C -> ident (seqType B * seqType C))
+        (spec : combType A -> combType C -> seqType B * seqType C)
+        input :
+    (forall a c, sequential (f ([a], [c])) = spec a c) ->
+    sequential (loop (CavaSeq:=SequentialSemantics) f input)
+    = fst (fold_left (fun loop_state t =>
+                        let '(acc, feedback) := loop_state in
+                        let a := nth t input (defaultCombValue A) in
+                        let c := hd (defaultCombValue C) feedback in
+                        let r := spec a c in
+                        (overlap t acc (fst r), overlap 0 (tl feedback) (snd r)))
+                     (seq 0 (length input))
+                     ([], [defaultCombValue C])).
+  Proof.
+    intros. erewrite loop_stepwise by eassumption.
+    erewrite fold_left_to_seq with (ls:=input) (default:=defaultCombValue A).
+    pose (R:=fun t (x : seqType B * seqType C) (y : nat * seqType B * seqType C) =>
+               y = (t, fst x, snd x)).
+    factor_out_loops.
+    lazymatch goal with
+    | |- ?P ?loop1 ?loop2 =>
+      let H := fresh in
+      assert (R (length input) loop1 loop2) as H;
+        (* prove that R implies postcondition *)
+        [ | subst R; cbv beta in *; rewrite H; reflexivity ]
+    end.
+    eapply fold_left_preserves_relation_seq with (R0:=R).
+    { (* R holds at start *)
+      reflexivity. }
+    { (* R holds through loop *)
+      subst R. cbv beta zeta.
+      intros. repeat destruct_pair_let. subst.
+      reflexivity. }
+  Qed.
+
+  Lemma loop_invariant {A B C}
+        (f : seqType A * seqType C -> ident (seqType B * seqType C))
+        (I : nat -> seqType B -> seqType C -> Prop)
+        (P : seqType B -> Prop) input :
+    (* invariant is true for start state *)
+    I 0 [] [defaultCombValue C] ->
+    (* invariant holds through loop *)
+    (forall t b c,
+        I t b c ->
+        t < length input ->
+        let a := nth t input (defaultCombValue A) in
+        let x := hd (defaultCombValue C) c in
+        let r := sequential (f ([a], [x])) in
+        I (S t) (overlap t b (fst r)) (overlap 0 (tl c) (snd r))) ->
+    (* invariant is strong enough to prove postcondition *)
+    (forall b c, I (length input) b c -> P b) ->
+    P (sequential (loop (CavaSeq:=SequentialSemantics) f input)).
+  Proof.
+    intros Hstart Hbody Hpost.
+    erewrite loop_stepwise_indexed by (intros; reflexivity).
+    cbv beta.
+    eapply fold_left_invariant_seq with
+        (I0:=fun t '(b,c) => I t b c).
+    { assumption. }
+    { intros *; repeat destruct_pair_let; intros.
+      seqsimpl. apply Hbody; eauto; lia. }
+    { intros *; repeat destruct_pair_let; intros.
+      eauto. }
+  Qed.
+
+  (* More flexible than loop_invariant about the start state satisfying the invariant *)
+  Lemma loop_invariant_alt {A B C}
+        (f : seqType A * seqType C -> ident (seqType B * seqType C))
+        (I : nat -> seqType B -> seqType C -> Prop)
+        (P : seqType B -> Prop) input :
+    (* Either the input is nil and P holds on nil, or the invariant is satisfied
+       after one step *)
+    (match input with
+     | [] => P []
+     | i0 :: _ =>
+       let r := sequential (f ([i0], [defaultCombValue C])) in
+       I 1 (fst r) (snd r)
+     end) ->
+    (* invariant holds through loop *)
+    (forall t b c,
+        I t b c ->
+        t < length input ->
+        let a := nth t input (defaultCombValue A) in
+        let x := hd (defaultCombValue C) c in
+        let r := sequential (f ([a], [x])) in
+        I (S t) (overlap t b (fst r)) (overlap 0 (tl c) (snd r))) ->
+    (* invariant is strong enough to prove postcondition *)
+    (forall b c, I (length input) b c -> P b) ->
+    P (sequential (loop (CavaSeq:=SequentialSemantics) f input)).
+  Proof.
+    intros Hstart Hbody Hpost.
+    erewrite loop_stepwise_indexed by (intros; reflexivity).
+    destruct input; [ cbn [fold_left]; seqsimpl; assumption | ].
+    cbn [fold_left seq length]. seqsimpl.
+    eapply fold_left_invariant_seq with
+        (I0:=fun t '(b,c) => I t b c).
+    { apply Hstart. }
+    { intros *; repeat destruct_pair_let; intros.
+      apply Hbody; eauto using in_cons; length_hammer. }
+    { intros *; repeat destruct_pair_let; intros.
+      eauto. }
+  Qed.
+End Loops.
